user 3, session 73, part 7

diffs-w-failures/3/user-3-session-73.v
@@ -12,4 +12,50 @@ Require Import Spec.Proc.
 Require Import Spec.Hoare.
 Unset Silent.
 Set Diffs "off".
-Timeout 1 Check @readNone.
+Set Printing Width 78.
+Set Silent.
+From Transitions Require Import Relations Rewriting NonError.
+Require Import Abstraction.
+Require Import Layer.
+Section Abstraction.
+Context (AState CState : Type).
+Context (absr : relation AState CState unit).
+Context (absr_ok : NonError absr).
+Definition refine_spec T R (spec : Specification T R AState) :
+  AState -> Specification T R CState :=
+  fun s cs =>
+  {|
+  pre := absr s (Val cs tt) /\ (spec s).(pre);
+  post := fun cs' r =>
+          exists s', absr s' (Val cs' tt) /\ (spec s).(post) s' r;
+  alternate := fun cs' r =>
+               exists s', absr s' (Val cs' tt) /\ (spec s).(alternate) s' r |}.
+Context A_Op C_Op `(a_sem : Dynamics A_Op AState)
+ `(c_sem : Dynamics C_Op CState).
+Import RelationNotations.
+Lemma proc_rspec_refine_exec T R (p : proc C_Op T) 
+  (rec : proc C_Op R) spec :
+  (forall t, proc_rspec c_sem p rec (refine_spec spec t)) ->
+  (forall sA sC, absr sA (Val sC tt) -> (spec sA).(pre)) ->
+  _ <- absr; exec c_sem p ---> v <- spec_exec spec; _ <- absr; pure v.
+Proof.
+(intros Hprspec Habstr_pre).
+Admitted.
+Lemma proc_rspec_refine_rec T R (p : proc C_Op T) 
+  (rec : proc C_Op R) spec :
+  (forall t, proc_rspec c_sem p rec (refine_spec spec t)) ->
+  (forall sA sC, absr sA (Val sC tt) -> (spec sA).(pre)) ->
+  _ <- absr; rexec c_sem p rec ---> v <- spec_aexec spec; _ <- absr; pure v.
+Proof.
+(intros Hprspec Habstr_pre).
+Admitted.
+Lemma proc_rspec_crash_refines T (p : proc C_Op T) 
+  (rec : proc C_Op unit) spec op :
+  (forall t, proc_rspec c_sem p rec (refine_spec spec t)) ->
+  (forall sO sT, absr sO sT tt -> (spec sO).(pre)) ->
+  spec_exec spec ---> exec a_sem (Call op) ->
+  spec_aexec spec
+  --->
+   a_sem.(crash_step) + (a_sem.(step) op;; a_sem.(crash_step)) ->
+  crash_refines absr c_sem p rec (a_sem.(step) op)
+    (a_sem.(crash_step) + (a_sem.(step) op;; a_sem.(crash_step))).
